Add more arguments to vec elim

theories/autosubst/GAST.v
@@ -31,7 +31,7 @@ Inductive term : Type :=
   | tvec : term -> term -> term
   | tvnil : term -> term
   | tvcons : term -> term -> term -> term
-  | tvec_elim : mode -> term -> term -> term -> term -> term
+  | tvec_elim : mode -> term -> term -> term -> term -> term -> term -> term
   | bot : term
   | bot_elim : mode -> term -> term -> term.
 
@@ -251,20 +251,26 @@ exact (eq_trans
 Qed.
 
 Lemma congr_tvec_elim {s0 : mode} {s1 : term} {s2 : term} {s3 : term}
-  {s4 : term} {t0 : mode} {t1 : term} {t2 : term} {t3 : term} {t4 : term}
-  (H0 : s0 = t0) (H1 : s1 = t1) (H2 : s2 = t2) (H3 : s3 = t3) (H4 : s4 = t4)
-  : tvec_elim s0 s1 s2 s3 s4 = tvec_elim t0 t1 t2 t3 t4.
+  {s4 : term} {s5 : term} {s6 : term} {t0 : mode} {t1 : term} {t2 : term}
+  {t3 : term} {t4 : term} {t5 : term} {t6 : term} (H0 : s0 = t0)
+  (H1 : s1 = t1) (H2 : s2 = t2) (H3 : s3 = t3) (H4 : s4 = t4) (H5 : s5 = t5)
+  (H6 : s6 = t6) :
+  tvec_elim s0 s1 s2 s3 s4 s5 s6 = tvec_elim t0 t1 t2 t3 t4 t5 t6.
 Proof.
 exact (eq_trans
          (eq_trans
             (eq_trans
                (eq_trans
-                  (eq_trans eq_refl
-                     (ap (fun x => tvec_elim x s1 s2 s3 s4) H0))
-                  (ap (fun x => tvec_elim t0 x s2 s3 s4) H1))
-               (ap (fun x => tvec_elim t0 t1 x s3 s4) H2))
-            (ap (fun x => tvec_elim t0 t1 t2 x s4) H3))
-         (ap (fun x => tvec_elim t0 t1 t2 t3 x) H4)).
+                  (eq_trans
+                     (eq_trans
+                        (eq_trans eq_refl
+                           (ap (fun x => tvec_elim x s1 s2 s3 s4 s5 s6) H0))
+                        (ap (fun x => tvec_elim t0 x s2 s3 s4 s5 s6) H1))
+                     (ap (fun x => tvec_elim t0 t1 x s3 s4 s5 s6) H2))
+                  (ap (fun x => tvec_elim t0 t1 t2 x s4 s5 s6) H3))
+               (ap (fun x => tvec_elim t0 t1 t2 t3 x s5 s6) H4))
+            (ap (fun x => tvec_elim t0 t1 t2 t3 t4 x s6) H5))
+         (ap (fun x => tvec_elim t0 t1 t2 t3 t4 t5 x) H6)).
 Qed.
 
 Lemma congr_bot : bot = bot.
@@ -333,9 +339,10 @@ Fixpoint ren_term (xi_term : nat -> nat) (s : term) {struct s} : term :=
   | tvcons s0 s1 s2 =>
       tvcons (ren_term xi_term s0) (ren_term xi_term s1)
         (ren_term xi_term s2)
-  | tvec_elim s0 s1 s2 s3 s4 =>
+  | tvec_elim s0 s1 s2 s3 s4 s5 s6 =>
       tvec_elim s0 (ren_term xi_term s1) (ren_term xi_term s2)
-        (ren_term xi_term s3) (ren_term xi_term s4)
+        (ren_term xi_term s3) (ren_term xi_term s4) (ren_term xi_term s5)
+        (ren_term xi_term s6)
   | bot => bot
   | bot_elim s0 s1 s2 =>
       bot_elim s0 (ren_term xi_term s1) (ren_term xi_term s2)
@@ -398,9 +405,10 @@ term :=
   | tvcons s0 s1 s2 =>
       tvcons (subst_term sigma_term s0) (subst_term sigma_term s1)
         (subst_term sigma_term s2)
-  | tvec_elim s0 s1 s2 s3 s4 =>
+  | tvec_elim s0 s1 s2 s3 s4 s5 s6 =>
       tvec_elim s0 (subst_term sigma_term s1) (subst_term sigma_term s2)
         (subst_term sigma_term s3) (subst_term sigma_term s4)
+        (subst_term sigma_term s5) (subst_term sigma_term s6)
   | bot => bot
   | bot_elim s0 s1 s2 =>
       bot_elim s0 (subst_term sigma_term s1) (subst_term sigma_term s2)
@@ -488,11 +496,13 @@ subst_term sigma_term s = s :=
       congr_tvcons (idSubst_term sigma_term Eq_term s0)
         (idSubst_term sigma_term Eq_term s1)
         (idSubst_term sigma_term Eq_term s2)
-  | tvec_elim s0 s1 s2 s3 s4 =>
+  | tvec_elim s0 s1 s2 s3 s4 s5 s6 =>
       congr_tvec_elim (eq_refl s0) (idSubst_term sigma_term Eq_term s1)
         (idSubst_term sigma_term Eq_term s2)
         (idSubst_term sigma_term Eq_term s3)
         (idSubst_term sigma_term Eq_term s4)
+        (idSubst_term sigma_term Eq_term s5)
+        (idSubst_term sigma_term Eq_term s6)
   | bot => congr_bot
   | bot_elim s0 s1 s2 =>
       congr_bot_elim (eq_refl s0) (idSubst_term sigma_term Eq_term s1)
@@ -584,11 +594,13 @@ ren_term xi_term s = ren_term zeta_term s :=
       congr_tvcons (extRen_term xi_term zeta_term Eq_term s0)
         (extRen_term xi_term zeta_term Eq_term s1)
         (extRen_term xi_term zeta_term Eq_term s2)
-  | tvec_elim s0 s1 s2 s3 s4 =>
+  | tvec_elim s0 s1 s2 s3 s4 s5 s6 =>
       congr_tvec_elim (eq_refl s0) (extRen_term xi_term zeta_term Eq_term s1)
         (extRen_term xi_term zeta_term Eq_term s2)
         (extRen_term xi_term zeta_term Eq_term s3)
         (extRen_term xi_term zeta_term Eq_term s4)
+        (extRen_term xi_term zeta_term Eq_term s5)
+        (extRen_term xi_term zeta_term Eq_term s6)
   | bot => congr_bot
   | bot_elim s0 s1 s2 =>
       congr_bot_elim (eq_refl s0) (extRen_term xi_term zeta_term Eq_term s1)
@@ -681,11 +693,13 @@ subst_term sigma_term s = subst_term tau_term s :=
       congr_tvcons (ext_term sigma_term tau_term Eq_term s0)
         (ext_term sigma_term tau_term Eq_term s1)
         (ext_term sigma_term tau_term Eq_term s2)
-  | tvec_elim s0 s1 s2 s3 s4 =>
+  | tvec_elim s0 s1 s2 s3 s4 s5 s6 =>
       congr_tvec_elim (eq_refl s0) (ext_term sigma_term tau_term Eq_term s1)
         (ext_term sigma_term tau_term Eq_term s2)
         (ext_term sigma_term tau_term Eq_term s3)
         (ext_term sigma_term tau_term Eq_term s4)
+        (ext_term sigma_term tau_term Eq_term s5)
+        (ext_term sigma_term tau_term Eq_term s6)
   | bot => congr_bot
   | bot_elim s0 s1 s2 =>
       congr_bot_elim (eq_refl s0) (ext_term sigma_term tau_term Eq_term s1)
@@ -787,12 +801,14 @@ Fixpoint compRenRen_term (xi_term : nat -> nat) (zeta_term : nat -> nat)
       congr_tvcons (compRenRen_term xi_term zeta_term rho_term Eq_term s0)
         (compRenRen_term xi_term zeta_term rho_term Eq_term s1)
         (compRenRen_term xi_term zeta_term rho_term Eq_term s2)
-  | tvec_elim s0 s1 s2 s3 s4 =>
+  | tvec_elim s0 s1 s2 s3 s4 s5 s6 =>
       congr_tvec_elim (eq_refl s0)
         (compRenRen_term xi_term zeta_term rho_term Eq_term s1)
         (compRenRen_term xi_term zeta_term rho_term Eq_term s2)
         (compRenRen_term xi_term zeta_term rho_term Eq_term s3)
         (compRenRen_term xi_term zeta_term rho_term Eq_term s4)
+        (compRenRen_term xi_term zeta_term rho_term Eq_term s5)
+        (compRenRen_term xi_term zeta_term rho_term Eq_term s6)
   | bot => congr_bot
   | bot_elim s0 s1 s2 =>
       congr_bot_elim (eq_refl s0)
@@ -900,12 +916,14 @@ subst_term tau_term (ren_term xi_term s) = subst_term theta_term s :=
       congr_tvcons (compRenSubst_term xi_term tau_term theta_term Eq_term s0)
         (compRenSubst_term xi_term tau_term theta_term Eq_term s1)
         (compRenSubst_term xi_term tau_term theta_term Eq_term s2)
-  | tvec_elim s0 s1 s2 s3 s4 =>
+  | tvec_elim s0 s1 s2 s3 s4 s5 s6 =>
       congr_tvec_elim (eq_refl s0)
         (compRenSubst_term xi_term tau_term theta_term Eq_term s1)
         (compRenSubst_term xi_term tau_term theta_term Eq_term s2)
         (compRenSubst_term xi_term tau_term theta_term Eq_term s3)
         (compRenSubst_term xi_term tau_term theta_term Eq_term s4)
+        (compRenSubst_term xi_term tau_term theta_term Eq_term s5)
+        (compRenSubst_term xi_term tau_term theta_term Eq_term s6)
   | bot => congr_bot
   | bot_elim s0 s1 s2 =>
       congr_bot_elim (eq_refl s0)
@@ -1036,12 +1054,14 @@ ren_term zeta_term (subst_term sigma_term s) = subst_term theta_term s :=
         (compSubstRen_term sigma_term zeta_term theta_term Eq_term s0)
         (compSubstRen_term sigma_term zeta_term theta_term Eq_term s1)
         (compSubstRen_term sigma_term zeta_term theta_term Eq_term s2)
-  | tvec_elim s0 s1 s2 s3 s4 =>
+  | tvec_elim s0 s1 s2 s3 s4 s5 s6 =>
       congr_tvec_elim (eq_refl s0)
         (compSubstRen_term sigma_term zeta_term theta_term Eq_term s1)
         (compSubstRen_term sigma_term zeta_term theta_term Eq_term s2)
         (compSubstRen_term sigma_term zeta_term theta_term Eq_term s3)
         (compSubstRen_term sigma_term zeta_term theta_term Eq_term s4)
+        (compSubstRen_term sigma_term zeta_term theta_term Eq_term s5)
+        (compSubstRen_term sigma_term zeta_term theta_term Eq_term s6)
   | bot => congr_bot
   | bot_elim s0 s1 s2 =>
       congr_bot_elim (eq_refl s0)
@@ -1174,12 +1194,14 @@ subst_term tau_term (subst_term sigma_term s) = subst_term theta_term s :=
         (compSubstSubst_term sigma_term tau_term theta_term Eq_term s0)
         (compSubstSubst_term sigma_term tau_term theta_term Eq_term s1)
         (compSubstSubst_term sigma_term tau_term theta_term Eq_term s2)
-  | tvec_elim s0 s1 s2 s3 s4 =>
+  | tvec_elim s0 s1 s2 s3 s4 s5 s6 =>
       congr_tvec_elim (eq_refl s0)
         (compSubstSubst_term sigma_term tau_term theta_term Eq_term s1)
         (compSubstSubst_term sigma_term tau_term theta_term Eq_term s2)
         (compSubstSubst_term sigma_term tau_term theta_term Eq_term s3)
         (compSubstSubst_term sigma_term tau_term theta_term Eq_term s4)
+        (compSubstSubst_term sigma_term tau_term theta_term Eq_term s5)
+        (compSubstSubst_term sigma_term tau_term theta_term Eq_term s6)
   | bot => congr_bot
   | bot_elim s0 s1 s2 =>
       congr_bot_elim (eq_refl s0)
@@ -1341,12 +1363,14 @@ Fixpoint rinst_inst_term (xi_term : nat -> nat) (sigma_term : nat -> term)
       congr_tvcons (rinst_inst_term xi_term sigma_term Eq_term s0)
         (rinst_inst_term xi_term sigma_term Eq_term s1)
         (rinst_inst_term xi_term sigma_term Eq_term s2)
-  | tvec_elim s0 s1 s2 s3 s4 =>
+  | tvec_elim s0 s1 s2 s3 s4 s5 s6 =>
       congr_tvec_elim (eq_refl s0)
         (rinst_inst_term xi_term sigma_term Eq_term s1)
         (rinst_inst_term xi_term sigma_term Eq_term s2)
         (rinst_inst_term xi_term sigma_term Eq_term s3)
         (rinst_inst_term xi_term sigma_term Eq_term s4)
+        (rinst_inst_term xi_term sigma_term Eq_term s5)
+        (rinst_inst_term xi_term sigma_term Eq_term s6)
   | bot => congr_bot
   | bot_elim s0 s1 s2 =>
       congr_bot_elim (eq_refl s0)
@@ -1611,11 +1635,14 @@ Fixpoint allfv_term (p_term : nat -> Prop) (s : term) {struct s} : Prop :=
   | tvcons s0 s1 s2 =>
       and (allfv_term p_term s0)
         (and (allfv_term p_term s1) (and (allfv_term p_term s2) True))
-  | tvec_elim s0 s1 s2 s3 s4 =>
+  | tvec_elim s0 s1 s2 s3 s4 s5 s6 =>
       and True
         (and (allfv_term p_term s1)
            (and (allfv_term p_term s2)
-              (and (allfv_term p_term s3) (and (allfv_term p_term s4) True))))
+              (and (allfv_term p_term s3)
+                 (and (allfv_term p_term s4)
+                    (and (allfv_term p_term s5)
+                       (and (allfv_term p_term s6) True))))))
   | bot => True
   | bot_elim s0 s1 s2 =>
       and True (and (allfv_term p_term s1) (and (allfv_term p_term s2) True))
@@ -1713,12 +1740,14 @@ Fixpoint allfvTriv_term (p_term : nat -> Prop) (H_term : forall x, p_term x)
       conj (allfvTriv_term p_term H_term s0)
         (conj (allfvTriv_term p_term H_term s1)
            (conj (allfvTriv_term p_term H_term s2) I))
-  | tvec_elim s0 s1 s2 s3 s4 =>
+  | tvec_elim s0 s1 s2 s3 s4 s5 s6 =>
       conj I
         (conj (allfvTriv_term p_term H_term s1)
            (conj (allfvTriv_term p_term H_term s2)
               (conj (allfvTriv_term p_term H_term s3)
-                 (conj (allfvTriv_term p_term H_term s4) I))))
+                 (conj (allfvTriv_term p_term H_term s4)
+                    (conj (allfvTriv_term p_term H_term s5)
+                       (conj (allfvTriv_term p_term H_term s6) I))))))
   | bot => I
   | bot_elim s0 s1 s2 =>
       conj I
@@ -2210,7 +2239,7 @@ allfv_term p_term s -> allfv_term q_term s :=
                                     end
                      end
                  end) I))
-  | tvec_elim s0 s1 s2 s3 s4 =>
+  | tvec_elim s0 s1 s2 s3 s4 s5 s6 =>
       fun HP =>
       conj I
         (conj
@@ -2260,7 +2289,50 @@ allfv_term p_term s -> allfv_term q_term s :=
                                    end
                                end
                            end
-                       end) I))))
+                       end)
+                    (conj
+                       (allfvImpl_term p_term q_term H_term s5
+                          match HP with
+                          | conj _ HP =>
+                              match HP with
+                              | conj _ HP =>
+                                  match HP with
+                                  | conj _ HP =>
+                                      match HP with
+                                      | conj _ HP =>
+                                          match HP with
+                                          | conj _ HP =>
+                                              match HP with
+                                              | conj HP _ => HP
+                                              end
+                                          end
+                                      end
+                                  end
+                              end
+                          end)
+                       (conj
+                          (allfvImpl_term p_term q_term H_term s6
+                             match HP with
+                             | conj _ HP =>
+                                 match HP with
+                                 | conj _ HP =>
+                                     match HP with
+                                     | conj _ HP =>
+                                         match HP with
+                                         | conj _ HP =>
+                                             match HP with
+                                             | conj _ HP =>
+                                                 match HP with
+                                                 | conj _ HP =>
+                                                     match HP with
+                                                     | conj HP _ => HP
+                                                     end
+                                                 end
+                                             end
+                                         end
+                                     end
+                                 end
+                             end) I))))))
   | bot => fun HP => I
   | bot_elim s0 s1 s2 =>
       fun HP =>
@@ -2755,7 +2827,7 @@ allfv_term (funcomp p_term xi_term) s :=
                                    end
                      end
                  end) I))
-  | tvec_elim s0 s1 s2 s3 s4 =>
+  | tvec_elim s0 s1 s2 s3 s4 s5 s6 =>
       fun H =>
       conj I
         (conj
@@ -2804,7 +2876,50 @@ allfv_term (funcomp p_term xi_term) s :=
                                    end
                                end
                            end
-                       end) I))))
+                       end)
+                    (conj
+                       (allfvRenL_term p_term xi_term s5
+                          match H with
+                          | conj _ H =>
+                              match H with
+                              | conj _ H =>
+                                  match H with
+                                  | conj _ H =>
+                                      match H with
+                                      | conj _ H =>
+                                          match H with
+                                          | conj _ H =>
+                                              match H with
+                                              | conj H _ => H
+                                              end
+                                          end
+                                      end
+                                  end
+                              end
+                          end)
+                       (conj
+                          (allfvRenL_term p_term xi_term s6
+                             match H with
+                             | conj _ H =>
+                                 match H with
+                                 | conj _ H =>
+                                     match H with
+                                     | conj _ H =>
+                                         match H with
+                                         | conj _ H =>
+                                             match H with
+                                             | conj _ H =>
+                                                 match H with
+                                                 | conj _ H =>
+                                                     match H with
+                                                     | conj H _ => H
+                                                     end
+                                                 end
+                                             end
+                                         end
+                                     end
+                                 end
+                             end) I))))))
   | bot => fun H => I
   | bot_elim s0 s1 s2 =>
       fun H =>
@@ -3300,7 +3415,7 @@ allfv_term p_term (ren_term xi_term s) :=
                                    end
                      end
                  end) I))
-  | tvec_elim s0 s1 s2 s3 s4 =>
+  | tvec_elim s0 s1 s2 s3 s4 s5 s6 =>
       fun H =>
       conj I
         (conj
@@ -3349,7 +3464,50 @@ allfv_term p_term (ren_term xi_term s) :=
                                    end
                                end
                            end
-                       end) I))))
+                       end)
+                    (conj
+                       (allfvRenR_term p_term xi_term s5
+                          match H with
+                          | conj _ H =>
+                              match H with
+                              | conj _ H =>
+                                  match H with
+                                  | conj _ H =>
+                                      match H with
+                                      | conj _ H =>
+                                          match H with
+                                          | conj _ H =>
+                                              match H with
+                                              | conj H _ => H
+                                              end
+                                          end
+                                      end
+                                  end
+                              end
+                          end)
+                       (conj
+                          (allfvRenR_term p_term xi_term s6
+                             match H with
+                             | conj _ H =>
+                                 match H with
+                                 | conj _ H =>
+                                     match H with
+                                     | conj _ H =>
+                                         match H with
+                                         | conj _ H =>
+                                             match H with
+                                             | conj _ H =>
+                                                 match H with
+                                                 | conj _ H =>
+                                                     match H with
+                                                     | conj H _ => H
+                                                     end
+                                                 end
+                                             end
+                                         end
+                                     end
+                                 end
+                             end) I))))))
   | bot => fun H => I
   | bot_elim s0 s1 s2 =>
       fun H =>
