theories/CastRemoval.v
@@ -35,7 +35,7 @@ Equations castrm : term → term := {
   ε| tvec A n | := tvec ε|A| ε|n| ;
   ε| tvnil A | := tvnil ε|A| ;
   ε| tvcons a n v | := tvcons ε|a| ε|n| ε|v| ;
-  ε| tvec_elim m v P z s | := tvec_elim m ε|v| ε|P| ε|z| ε|s| ;
+  ε| tvec_elim m A n v P z s | := tvec_elim m ε|A| ε|n| ε|v| ε|P| ε|z| ε|s| ;
   ε| bot | := bot ;
   ε| bot_elim m A p | := bot_elim m ε|A| ε|p|
 }
