theories/Revival.v
@@ -57,8 +57,16 @@ Equations revive_term (Γ : scope) (t : term) : cterm := {
   ⟦ Γ | tnat_elim m n P z s ⟧v :=
     if isGhost m then enat_elim ⟦ Γ | n ⟧ε ⟦ Γ | P ⟧ε ⟦ Γ | z ⟧v ⟦ Γ | s ⟧v
     else cDummy ;
-  ⟦ Γ | tvec_elim m v P z s ⟧v :=
-    if isGhost m then evec_elim ⟦ Γ | v ⟧ε ⟦ Γ | P ⟧ε ⟦ Γ | z ⟧v ⟦ Γ | s ⟧v
+  ⟦ Γ | tvec_elim m A n v P z s ⟧v :=
+    if isGhost m then (
+      (* We need to pass n as argument to s *)
+      let s' :=
+        clam cType ⟦ Γ | A ⟧τ (
+          capp (capp (S ⋅ ⟦ Γ | s ⟧v) (cvar 0)) (S ⋅ ⟦ Γ | n ⟧v)
+        )
+      in
+      evec_elim ⟦ Γ | v ⟧ε ⟦ Γ | P ⟧ε ⟦ Γ | z ⟧v s'
+    )
     else cDummy ;
   ⟦ Γ | bot_elim m A p ⟧v := if isGhost m then ⟦ Γ | A ⟧∅ else cDummy ;
   ⟦ _ | _ ⟧v := cDummy
@@ -238,7 +246,9 @@ Proof.
     + apply scoping_to_rev. apply erase_scoping.
     + apply scoping_to_rev. apply erase_scoping.
   - cbn. destruct_if e. 2: constructor.
-    escope. all: apply scoping_to_rev. all: apply erase_scoping.
+    escope. 5: reflexivity.
+    4,5: eapply cscoping_ren ; eauto using crscoping_S.
+    all: apply scoping_to_rev. all: apply erase_scoping.
   - cbn.
     destruct_if e. 2: constructor.
     constructor. eapply scoping_to_rev. eapply erase_scoping.
@@ -298,9 +308,9 @@ Proof.
     erewrite !erase_ren. 2-5: eassumption.
     reflexivity.
   - cbn. destruct_ifs. 2: eauto.
-    cbn. erewrite IHt3, IHt4. 2-5: eassumption.
-    erewrite !erase_ren. 2-5: eassumption.
-    reflexivity.
+    cbn. erewrite IHt2, IHt5, IHt6. 2-7: eassumption.
+    erewrite !erase_ren. 2-7: eassumption.
+    f_equal. f_equal. ssimpl. reflexivity.
   - cbn.
     destruct_ifs. 2: eauto.
     erewrite erase_ren. 2,3: eassumption.
@@ -435,13 +445,11 @@ Proof.
     rewrite !erase_rev_subst.
     destruct_if eg. 2: reflexivity.
     reflexivity.
-  - cbn.
-    erewrite IHt3. 2,3: eassumption.
-    erewrite IHt4. 2,3: eassumption.
-    erewrite !erase_subst. 2-5: eassumption.
+  - cbn. erewrite IHt2, IHt5, IHt6. 2-7: eassumption.
+    erewrite !erase_subst. 2-7: eassumption.
     rewrite !erase_rev_subst.
     destruct_if eg. 2: reflexivity.
-    reflexivity.
+    cbn. f_equal. f_equal. ssimpl. reflexivity.
   - cbn.
     destruct_ifs. 2: reflexivity.
     erewrite erase_subst. 2,3: eassumption.
@@ -554,8 +562,17 @@ Proof.
       constructor.
   - cbn. remd. cbn. destruct_if eg. 2: constructor.
     mode_eqs. cbn. eapply cconv_trans. 1: constructor.
-    apply ccmeta_refl. f_equal.
-    admit.
+    eapply cconv_trans.
+    1:{
+      econstructor. 2: econv.
+      econstructor. 2: econv.
+      constructor.
+    }
+    cbn. lhs_ssimpl.
+    econv.
+    + eapply cconv_trans. 1: constructor.
+      cbn.
+    +
   - cbn.
     cbn in IHh2, IHh3.
     eapply conv_md in h3 as e3. simpl in e3. rewrite <- e3.
